typed HOL

translation.v
@@ -441,12 +441,12 @@ Qed.
 (** Typed HOL deduction system **)
 
 Inductive THOL_prv (Xi : list sort) (A : list form) : form -> Prop :=
-| THOL_CTX phi : In phi A -> THOL_prv Xi A phi
-| THOL_II phi psi : THOL_prv Xi (phi :: A) psi -> THOL_prv Xi A (implies phi psi)
+| THOL_CTX phi : In phi A -> is_prop Xi phi -> THOL_prv Xi A phi
+| THOL_II phi psi : THOL_prv Xi (phi :: A) psi -> is_prop Xi phi -> THOL_prv Xi A (implies phi psi)
 | THOL_IE phi psi : THOL_prv Xi A (implies phi psi) -> THOL_prv Xi A phi -> THOL_prv Xi A psi
 | THOL_AI phi s : THOL_prv (s :: Xi) (map (ren_form ↑) A) phi -> THOL_prv Xi A (all s phi)
 | THOL_AE phi s p : THOL_prv Xi A (all s phi) -> has_sort Xi p s -> THOL_prv Xi A phi[p..]
-| THOL_CI phi s p : THOL_prv Xi A phi[p..] -> THOL_prv Xi A (holds (cterm s phi) p)
+| THOL_CI phi s p : THOL_prv Xi A phi[p..] -> has_sort Xi p s -> THOL_prv Xi A (holds (cterm s phi) p)
 | THOL_CE phi s p : THOL_prv Xi A (holds (cterm s phi) p) -> THOL_prv Xi A phi[p..].
 
 Lemma THOL_weak Xi A A' phi :
@@ -456,10 +456,143 @@ Proof.
   all: try unshelve (solve [econstructor; auto with datatypes]); try now econstructor.
 Qed.
 
-Lemma THOL_is_prop Xi A phi :
-  (forall psi, In psi A -> is_prop Xi psi) -> THOL_prv Xi A phi -> is_prop Xi phi.
+Lemma is_prop_ren Xi Xi' phi sigma :
+  is_prop Xi phi
+  -> (forall n s, lup Xi n = Some s -> lup Xi' (sigma n) = Some s)
+  -> is_prop Xi' phi⟨sigma⟩
+with has_sort_ren Xi Xi' t s sigma :
+  has_sort Xi t s
+  -> (forall n s, lup Xi n = Some s -> lup Xi' (sigma n) = Some s)
+  -> has_sort Xi' t⟨sigma⟩ s.
 Proof.
-Admitted.
+  induction 1 in Xi', sigma |- *; intros HS; cbn.
+  - constructor; eauto.
+  - constructor. apply IHis_prop. intros [] s'; cbn; eauto.
+  - fold ren_term. apply ip_holds with s.
+    + eapply has_sort_ren; eauto.
+    + eapply has_sort_ren; eauto.
+  - induction 1 in Xi', sigma |- *; intros HS; cbn.
+    + apply hs_var. now apply HS.
+    + fold ren_form. constructor. eapply is_prop_ren; eauto.
+      intros [] s'; cbn; eauto.
+Qed.
+
+Lemma is_prop_subst Xi Xi' phi sigma :
+  is_prop Xi phi
+  -> (forall n s, lup Xi n = Some s -> has_sort Xi' (sigma n) s)
+  -> is_prop Xi' phi[sigma]
+with has_sort_subst Xi Xi' t s sigma :
+  has_sort Xi t s
+  -> (forall n s, lup Xi n = Some s -> has_sort Xi' (sigma n) s)
+  -> has_sort Xi' t[sigma] s.
+Proof.
+  induction 1 in Xi', sigma |- *; intros HS; cbn.
+  - constructor; eauto.
+  - constructor. apply IHis_prop. intros [] s'; cbn.
+    + intros [=]; subst. now apply hs_var.
+    + intros H'. eapply has_sort_ren; eauto.
+  - fold subst_term. apply ip_holds with s.
+    + eapply has_sort_subst; eauto.
+    + eapply has_sort_subst; eauto.
+  - induction 1 in Xi', sigma |- *; intros HS; cbn.
+    + now apply HS.
+    + fold subst_form. constructor. eapply is_prop_subst; eauto.
+      intros [] s'; cbn.
+      * intros [=]; subst. now apply hs_var.
+      * intros H'. eapply has_sort_ren; eauto.
+Qed.
+
+Lemma is_prop_ren' Xi Xi' phi sigma :
+  (forall n s, lup Xi n = Some s <-> lup Xi' (sigma n) = Some s)
+  -> is_prop Xi phi <-> is_prop Xi' phi⟨sigma⟩
+with has_sort_ren' Xi Xi' t s sigma :
+  (forall n s, lup Xi n = Some s <-> lup Xi' (sigma n) = Some s)
+  -> has_sort Xi t s <-> has_sort Xi' t⟨sigma⟩ s.
+Proof.
+  induction phi in Xi, Xi', sigma |-*; intros HS; cbn; split; inversion 1; subst.
+  - constructor. eapply IHphi1; trivial. eapply IHphi2; trivial.
+  - constructor. eapply IHphi1; trivial. eapply IHphi2; trivial.
+  - constructor. eapply IHphi; eauto. intros [] s'; cbn; eauto. tauto.
+  - constructor. eapply IHphi; eauto. intros [] s'; cbn; eauto. tauto.
+  - fold ren_term. apply ip_holds with s.
+    + rewrite <- has_sort_ren'; eauto.
+    + rewrite <- has_sort_ren'; eauto.
+  - fold ren_term. apply ip_holds with s.
+    + rewrite has_sort_ren'; eauto.
+    + rewrite has_sort_ren'; eauto.
+  - induction t in Xi, Xi', sigma |- *; intros HS; cbn; split; inversion 1; subst.
+    + apply hs_var. now apply HS.
+    + apply hs_var. now apply HS.
+    + fold ren_form. constructor. rewrite <- is_prop_ren'; eauto.
+      intros [] s'; cbn; eauto. tauto.
+    + fold ren_form. constructor. rewrite is_prop_ren'; eauto.
+      intros [] s'; cbn; eauto. tauto.
+Qed.
+
+Lemma is_prop_subst' Xi Xi' phi sigma :
+  (forall n s, lup Xi n = Some s <-> has_sort Xi' (sigma n) s)
+  -> is_prop Xi phi <-> is_prop Xi' phi[sigma]
+with has_sort_subst' Xi Xi' t s sigma :
+  (forall n s, lup Xi n = Some s <-> has_sort Xi' (sigma n) s)
+  -> has_sort Xi t s <-> has_sort Xi' t[sigma] s.
+Proof.
+  induction phi in Xi, Xi', sigma |-*; intros HS; cbn; split; inversion 1; subst.
+  - constructor. eapply IHphi1; trivial. eapply IHphi2; trivial.
+  - constructor. eapply IHphi1; trivial. eapply IHphi2; trivial.
+  - constructor. eapply IHphi; eauto. intros [] s'; cbn; split.
+    + intros [=]; subst. now apply hs_var.
+    + inversion 1; subst. cbn in *. congruence.
+    + unfold funcomp. rewrite <- has_sort_ren'; try now apply HS. reflexivity.
+    + unfold funcomp. rewrite <- has_sort_ren'; try now apply HS. reflexivity.
+  - constructor. eapply IHphi; eauto. intros [] s'; cbn; split.
+    + intros [=]; subst. now apply hs_var.
+    + inversion 1; subst. cbn in *. congruence.
+    + unfold funcomp. rewrite <- has_sort_ren'; try now apply HS. reflexivity.
+    + unfold funcomp. rewrite <- has_sort_ren'; try now apply HS. reflexivity.
+  - fold subst_term. econstructor; rewrite <- has_sort_subst'; eauto.
+  - fold subst_term in *. econstructor; rewrite -> has_sort_subst'; eauto.
+  - induction t in Xi, Xi', sigma |-*; intros HS; cbn; split; inversion 1; subst.
+    + now apply HS.
+    + apply hs_var. apply HS. rewrite <- H0. now apply hs_var.
+    + apply hs_var. apply HS. rewrite <- H0. now constructor.
+    + fold subst_form. constructor. rewrite <- is_prop_subst'; eauto.
+      intros [] s'; cbn; split.
+      * intros [=]; subst. now apply hs_var.
+      * inversion 1; subst. cbn in *. congruence.
+      * unfold funcomp. rewrite <- has_sort_ren'. apply HS. reflexivity.
+      * unfold funcomp. rewrite <- has_sort_ren'. apply HS. reflexivity.
+    + fold subst_form in *. constructor. rewrite is_prop_subst'; eauto.
+      intros [] s'; cbn; split.
+      * intros [=]; subst. now apply hs_var.
+      * inversion 1; subst. cbn in *. congruence.
+      * unfold funcomp. rewrite <- has_sort_ren'. apply HS. reflexivity.
+      * unfold funcomp. rewrite <- has_sort_ren'. apply HS. reflexivity.
+Qed.
+
+Lemma has_sort_unique Xi t s s' :
+  has_sort Xi t s -> has_sort Xi t s' -> s = s'.
+Proof.
+  induction 1; cbn; inversion 1; subst; congruence.
+Qed.
+
+Lemma THOL_is_prop Xi A phi :
+  THOL_prv Xi A phi -> is_prop Xi phi.
+Proof.
+  induction 1; trivial; try constructor; trivial.
+  - now inversion IHTHOL_prv1; subst.
+  - inversion IHTHOL_prv; subst.
+    eapply is_prop_subst; eauto.
+    intros [] s'; cbn; try apply hs_var. now intros [=]; subst.
+  - econstructor; eauto. constructor. eapply is_prop_subst'; eauto.
+    intros [] s'; cbn; split.
+    + now intros [=]; subst.
+    + intros H'. f_equal. eapply has_sort_unique; eauto.
+    + apply hs_var.
+    + now inversion 1; subst.
+  - inversion IHTHOL_prv; subst. inversion H2; subst.
+    eapply is_prop_subst; eauto.
+    intros [] s'; cbn; try apply hs_var. now intros [=]; subst.
+Qed.
 
 
 
@@ -1139,6 +1272,15 @@ Proof.
 Qed.
 
 Print Assumptions soundness'.
+
+Lemma soundness_typing_check Xi Psi psi p :
+  is_prop Xi psi
+  -> has_type Xi (map trans_T Psi) p (comp (trans_T psi))
+  -> is_spec Xi (map trans_T Psi) (trans_IL Xi) (after p (trans_S psi (var_prog 0))).
+Proof.
+  intros H1 H2. eapply is_after; eauto.
+  apply trans_is_spec; trivial. now apply ht_var.
+Qed.
 
 Theorem soundness Xi Psi psi :
   THOL_prv Xi Psi psi
